src/Refinements/LoggedDisk/Definitions.v
@@ -2,7 +2,10 @@ Require Import Framework CachedDiskLayer LoggedDiskLayer LogCache.Definitions.
 Close Scope pred_scope.
 Import ListNotations.
 
-Fixpoint compile {T} (p2: LoggedDiskHL.Lang.prog T) : CachedDiskHL.Lang.prog T.
+Notation "'low'" := CachedDiskLang.
+Notation "'high'" := LoggedDiskLang.
+
+Fixpoint compile {T} (p2: prog high T) : prog low T.
   destruct p2; simpl in *.
   {
     destruct p.
@@ -10,56 +13,57 @@ Fixpoint compile {T} (p2: LoggedDiskHL.Lang.prog T) : CachedDiskHL.Lang.prog T.
     exact (write l l0).
   }
   {
-    exact (CachedDiskHL.Lang.Ret t).
+    exact (Ret t).
   }
   {
-    exact (CachedDiskHL.Lang.Bind (compile T p2) (fun x => compile T' (p x))).
+    exact (Bind (compile T p2) (fun x => compile T' (p x))).
   }
 Defined.
 
-
-Fixpoint oracle_refines_to T (d1: State cached_disk_lts) (p: Prog logged_disk_lts T)  (o1: Oracle cached_disk_lts) (o2: Oracle logged_disk_lts) : Prop :=
-  CachedDiskHL.Lang.oracle_ok (compile p) o1 d1 /\
+Fixpoint oracle_refines_to T (d1: state low) (p: prog high T) o1 o2 : Prop :=
     match p with
-    | @Bind T1 T2 p1 p2 =>
-      exists o1' o1'',
+    | @Bind _ T1 T2 p1 p2 =>
+      exists o1' o1'' o2' o2'',
       o1 = o1'++o1'' /\
-     ((exists d1', CachedDiskHL.Lang.exec o1 d1 (compile p1) (Crashed d1') /\
-         oracle_refines_to T1 d1 p1 o1 o2) \/
+      o2 = o2' ++ o2'' /\
+     ((exists d1', exec low o1' d1 (compile p1) (Crashed d1') /\
+         oracle_refines_to T1 d1 p1 o1' o2') \/
       (exists d1' r ret,
-         CachedDiskHL.Lang.exec o1' d1 (compile p1) (Finished d1' r) /\
-         CachedDiskHL.Lang.exec o1'' d1' (compile (p2 r)) ret /\
-         exists o2' o2'',
+         exec low o1' d1 (compile p1) (Finished d1' r) /\
+         exec low o1'' d1' (compile (p2 r)) ret /\
          oracle_refines_to T1 d1 p1 o1' o2' /\
-         oracle_refines_to T2 d1' (p2 r) o1'' o2'' /\
-         o2 = o2' ++ o2''))
-    |Op op =>
+         oracle_refines_to T2 d1' (p2 r) o1'' o2''
+         ))
+    |Op _ op =>
      match op with
      | Read a =>
        (exists d1',
-          CachedDiskHL.Lang.exec o1 d1 (read a) (Crashed d1') /\
-          o2 = [OpOracle [CrashBefore] ]) \/
+          exec low o1 d1 (read a) (Crashed d1') /\
+          o2 = [OpOracle LoggedDiskOperation [CrashBefore] ]) \/
        (exists d1' r,
-          CachedDiskHL.Lang.exec o1 d1 (read a) (Finished d1' r) /\
-          o2 = [Cont])
+          exec low o1 d1 (read a) (Finished d1' r) /\
+          o2 = [OpOracle LoggedDiskOperation [LoggedDiskLayer.Definitions.Cont] ])
          
      | Write la lv =>
        (exists d1',
-          CachedDiskHL.Lang.exec o1 d1 (write la lv) (Crashed d1') /\
-          ((d1' = d1 /\ o2 = [ OpOracle [CrashBefore] ]) \/
-           (d1' <> d1 /\ o2 = [ OpOracle [CrashAfter] ]))) \/
+          exec low o1 d1 (write la lv) (Crashed d1') /\
+          ((d1' = d1 /\
+           o2 = [ OpOracle LoggedDiskOperation [CrashBefore] ]) \/
+           (d1' <> d1 /\
+            o2 = [ OpOracle LoggedDiskOperation [CrashAfter] ]))) \/
        (exists d1' r,
-          CachedDiskHL.Lang.exec o1 d1 (write la lv) (Finished d1' r) /\          
-          o2 = [Cont])
+          exec low o1 d1 (write la lv) (Finished d1' r) /\          
+          o2 = [OpOracle LoggedDiskOperation [LoggedDiskLayer.Definitions.Cont] ] /\
+       (forall s ,(exists F, cached_log_rep F s d1) -> (exists F, cached_log_rep F (write_all s la lv) d1')))
      end
 
     | Ret v =>
       (exists d1',
-         CachedDiskHL.Lang.exec o1 d1 (CachedDiskHL.Lang.Ret v) (Crashed d1') /\
-         o2 = [Crash]) \/
+         exec low o1 d1 (Ret v) (Crashed d1') /\
+         o2 = [Crash _]) \/
       (exists d1' r,
-         CachedDiskHL.Lang.exec o1 d1 (CachedDiskHL.Lang.Ret v) (Finished d1' r) /\
-         o2 = [Cont])
+         exec low o1 d1 (Ret v) (Finished d1' r) /\
+         o2 = [Language.Cont _])
     end
 .
 (*
@@ -91,8 +95,10 @@ Fixpoint oracle_refines_to T (d1: State cached_disk_lts) (p: Prog logged_disk_lt
         o2 = [Cont]
     end.
 *)
-  Definition refines_to (d1: State cached_disk_lts) (d2: State logged_disk_lts) :=
+  Definition refines_to (d1: state low) (d2: state high) :=
     exists F, cached_log_rep F d2 d1.
 
-  Definition compilation_of T (p1: Prog cached_disk_lts T) (p2: Prog logged_disk_lts T) :=
+  Definition compilation_of T (p1: prog low T) (p2: prog high T) :=
     p1 = @compile T p2.
+
+  Definition LoggedDiskRefinement := Build_Refinement compilation_of refines_to oracle_refines_to.
