src/Implementations/File/Definitions.v
@@ -1,0 +1,64 @@
+Require Import Framework LoggedDiskLayer Inode.
+
+Open Scope pred_scope.
+
+Record File :=
+  {
+    owner: user;
+    blocks: list value;
+  }.
+
+Definition file_rep file (inode: Inode) : @pred addr addr_dec (set value) :=
+  exists* fblocks,
+  [[ file.(owner) = inode.(Inode.Definitions.owner) ]] *
+  inode.(Inode.Definitions.blocks) |L> fblocks *
+  [[ file.(blocks) = map fst fblocks ]].
+
+Fixpoint file_list_inner_rep flist ilist :=
+  match flist, ilist with
+  | file::flist', inode::ilist' =>
+    file_rep file inode * file_list_inner_rep flist' ilist'
+  | _, _ => emp
+  end.
+
+Definition file_list_rep flist :=
+  exists* ilist,
+    inode_list_rep ilist *
+    let valid_ilist := filter (fun inode => inode.(used)) ilist in
+    [[ length flist = length valid_ilist ]] *
+    file_list_inner_rep flist valid_ilist.
+
+
+Definition read inum off :=
+  inode <- get_inode inum;
+  let bn := nth off inode.(Inode.Definitions.blocks) 0 in
+  v <-| Read bn;
+  Ret v.
+
+Definition write inum off v :=
+  inode <- get_inode inum;
+  let bn := nth off inode.(Inode.Definitions.blocks) 0 in
+  _ <-| Write [bn] [v];
+  Ret tt.
+
+Definition set_owner inum owner :=
+  inode <- get_inode inum;
+  let new_inode := Build_Inode inode.(used) owner inode.(Inode.Definitions.blocks) in
+  _ <- set_inode inum new_inode;
+  Ret tt.
+
+Definition create owner :=
+  minum <- get_last_unused_inum;
+  match minum with
+  | Some inum =>
+    _ <- set_inode inum (Build_Inode true owner []);
+    Ret (Some inum)
+  | None =>
+    Ret None
+  end.
+
+Definition delete inum :=
+  inode <- get_inode inum;
+  let new_inode := Build_Inode false inode.(Inode.Definitions.owner) [] in
+  _ <- set_inode inum new_inode;
+  Ret tt.
