src/Implementations/Inode/Definitions.v
@@ -1,0 +1,72 @@
+Require Import Framework LoggedDiskLayer.
+
+(* For simplicity, it will be 1 inode per block *)
+Axiom inode_count: nat.
+
+Definition Inum := addr.
+
+Record Inode :=
+  {
+    used : bool;
+    owner: user;
+    blocks : list addr;
+  }.
+
+Variable encode_inode : Inode -> value.
+Variable decode_inode: value -> Inode.
+Axiom inode_encode_decode:
+  forall i,
+    decode_inode (encode_inode i) = i.
+Axiom inode_decode_encode:
+  forall b,
+    encode_inode (decode_inode b) = b.
+
+Open Scope pred_scope.
+
+Definition inode_list_rep ilist : @pred addr addr_dec (set value) :=
+  exists* inode_blocks,
+  0 |=> inode_blocks *
+  [[ length inode_blocks = inode_count ]] *
+  [[ ilist = map (fun bs => decode_inode (fst bs)) inode_blocks ]].
+
+Definition get_inode inum :=
+  i <-| Read inum;
+  Ret (decode_inode i).
+
+Fixpoint get_last_unused_inum_rec n :=
+  match n with
+  | 0 =>
+    Ret None
+  | S n' =>
+    inode <- get_inode n';
+    if inode.(used) then
+      un <- get_last_unused_inum_rec n';
+      Ret un
+    else
+      Ret (Some n')
+end.
+
+Definition get_last_unused_inum :=
+  inum <- get_last_unused_inum_rec inode_count;
+  Ret inum.
+
+Definition set_inode inum inode:=
+  _ <-| Write [inum] [encode_inode inode];
+  Ret tt.
+
+
+
+
+
+
+
+
+
+
+
+
+
+
+
+
+
