src/Layers/FileLayer/Definitions.v
@@ -1,0 +1,299 @@
+Require Import Framework Inode File.
+Import ListNotations.
+Close Scope pred_scope.
+
+Set Implicit Arguments.
+  
+  Inductive token' :=
+  | CrashBefore : token'
+  | CrashAfter : token'
+  | CrashAfterCreate : Inum -> token'
+  | NewInum : Inum -> token'
+  | DiskFull : token'
+  | Cont : token'.
+
+  Definition token_dec' : forall (t t': token'), {t=t'}+{t<>t'}.
+    decide equality.
+    all: apply  addr_dec.
+  Defined.
+
+  Definition oracle' := list token'.  
+
+  Definition state' := disk File.
+  
+  Inductive prog' : Type -> Type :=
+  | Read : Inum -> addr -> prog' value
+  | Write : Inum -> addr -> value -> prog' unit
+  | Extend : Inum -> nat -> prog (option unit) 
+  | SetOwner : Inum -> user -> prog' unit
+  | Create : user -> prog' (option addr)
+  | Delete : Inum -> prog' unit.
+   
+  Inductive exec' :
+    forall T, oracle' ->  state' -> prog' T -> @Result state' T -> Prop :=
+  | ExecRead : 
+      forall d inum off file v,
+        d inum = Some file ->
+        nth_error file.(blocks) off = Some v ->
+        exec' [Cont] d (Read inum off) (Finished d v)
+             
+  | ExecWrite :
+      forall d inum file off v,
+        d inum = Some file ->
+        let new_file := Build_File file.(owner) (firstn off file.(blocks) ++ v :: skipn (S off) file.(blocks)) in
+        exec' [Cont] d (Write inum off v) (Finished (upd d inum new_file) tt)
+
+  | ExecSetOwner :
+      forall d inum file u,
+        d inum = Some file ->
+        let new_file := Build_File u file.(blocks) in
+        exec' [Cont] d (SetOwner inum u) (Finished (upd d inum new_file) tt)
+
+  | ExecCreateSuccess :
+      forall d inum u,
+        inum < Definitions.inode_count ->
+        d inum = None ->
+        let new_file := Build_File u [] in
+        exec' [NewInum inum] d (Create u) (Finished (upd d inum new_file) (Some inum))
+
+  | ExecCreateFail :
+      forall d u,
+        (forall inum, inum < Definitions.inode_count -> d inum <> None) ->
+        exec' [DiskFull] d (Create u) (Finished d None)
+              
+  | ExecDelete :
+      forall d inum file,
+        d inum = Some file ->
+        exec' [Cont] d (Delete inum) (Finished (Mem.delete d inum) tt)
+
+  | ExecCrashBefore :
+      forall d T (p: prog' T),
+        exec' [CrashBefore] d p (Crashed d)
+
+  | ExecWriteCrashAfter :
+      forall d inum file off v,
+        d inum = Some file ->
+        let new_file := Build_File file.(owner) (firstn off file.(blocks) ++ v :: skipn (S off) file.(blocks)) in
+        exec' [CrashAfter] d (Write inum off v) (Crashed (upd d inum new_file))
+
+  | ExecSetOwnerCrashAfter :
+      forall d inum file u,
+        d inum = Some file ->
+        let new_file := Build_File u file.(blocks) in
+        exec' [CrashAfter] d (SetOwner inum u) (Crashed (upd d inum new_file))
+
+  | ExecCreateCrashAfter :
+      forall d inum u,
+        d inum = None ->
+        let new_file := Build_File u [] in
+        exec' [CrashAfterCreate inum] d (Create u) (Finished (upd d inum new_file) (Some inum))
+
+  | ExecDeleteCrashAfter :
+      forall d inum file,
+        d inum = Some file ->
+        exec' [CrashAfter] d (Delete inum) (Finished (Mem.delete d inum) tt).
+
+  Hint Constructors exec' : core.
+
+   Definition weakest_precondition' T (p: prog' T) :=
+   match p in prog' T' return (T' -> state' -> Prop) -> oracle' -> state' -> Prop with
+   | Read inum a =>
+     (fun Q o s =>
+       exists file v,
+         o = [Cont] /\
+         s inum = Some file /\
+         nth_error file.(blocks) a = Some v /\
+         Q v s)
+   | Write inum a v =>
+     (fun Q o s =>
+        exists file,
+        o = [Cont] /\
+        s inum = Some file /\
+        let new_file :=
+            Build_File file.(owner)
+            (firstn a file.(blocks) ++ v :: skipn (S a) file.(blocks)) in
+        Q tt (upd s inum new_file))
+   | SetOwner inum u =>
+     (fun Q o s =>
+        exists file,
+        o = [Cont] /\
+        s inum = Some file /\
+        let new_file :=
+            Build_File u file.(blocks) in
+        Q tt (upd s inum new_file))
+   | Create u =>
+     (fun Q o s =>
+        (forall inum,
+           o = [DiskFull] /\
+           (inum < Definitions.inode_count -> s inum <> None) /\
+           Q None s) \/
+        (exists inum,
+           o = [NewInum inum] /\
+           inum < Definitions.inode_count /\ 
+           s inum = None /\
+           let new_file := Build_File u [] in
+           Q (Some inum) (upd s inum new_file)))
+     | Delete inum =>
+       (fun Q o s =>
+        exists file,
+        o = [Cont] /\
+        s inum = Some file /\
+        Q tt (Mem.delete s inum))
+   end.
+
+   Definition weakest_crash_precondition' T (p: prog' T) :=
+    match p in prog' T' return (state' -> Prop) -> oracle' -> state' -> Prop with
+   | Read a =>
+     (fun Q o s =>
+         o = [CrashBefore] /\
+         Q s)
+   | Write la lv =>
+     (fun Q o s =>
+       (o = [CrashBefore] /\
+        Q s) \/
+       (o = [CrashAfter] /\
+        Q (write_all s la lv)))
+    end.
+
+  Definition strongest_postcondition' T (p: prog' T) :=
+   match p in prog' T' return (oracle' -> state' -> Prop) -> T' -> state' -> Prop with
+   | Read inum a =>
+     (fun Q o s =>
+       exists file v,
+         o = [Cont] /\
+         s inum = Some file /\
+         nth_error file.(blocks) a = Some v /\
+         Q v s)
+   | Write inum a v =>
+     (fun Q o s =>
+        exists file,
+        o = [Cont] /\
+        s inum = Some file /\
+        let new_file :=
+            Build_File file.(owner)
+            (firstn a file.(blocks) ++ v :: skipn (S a) file.(blocks)) in
+        Q tt (upd s inum new_file))
+   | SetOwner inum u =>
+     (fun Q o s =>
+        exists file,
+        o = [Cont] /\
+        s inum = Some file /\
+        let new_file :=
+            Build_File u file.(blocks) in
+        Q tt (upd s inum new_file))
+   | Create u =>
+     (fun Q o s =>
+        (forall inum,
+           o = [DiskFull] /\
+           (inum < Definitions.inode_count -> s inum <> None) /\
+           Q None s) \/
+        (exists inum,
+           o = [NewInum inum] /\
+           inum < Definitions.inode_count /\ 
+           s inum = None /\
+           let new_file := Build_File u [] in
+           Q (Some inum) (upd s inum new_file)))
+     | Delete inum =>
+       (fun Q o s =>
+        exists file,
+        o = [Cont] /\
+        s inum = Some file /\
+        Q tt (Mem.delete s inum))
+   end.
+
+  Definition strongest_crash_postcondition' T (p: prog' T) :=
+    match p in prog' T' return (oracle' -> state' -> Prop) -> state' -> Prop with
+   | Read a =>
+     fun P s' =>
+       P [CrashBefore] s'
+   | Write la lv =>
+     fun P s' =>
+       (P [CrashBefore] s') \/
+       (exists s,
+          P [CrashAfter] s /\
+          s' = write_all s la lv)
+    end.
+  
+  Theorem sp_complete':
+    forall T (p: prog' T) P (Q: _ -> _ -> Prop),
+      (forall t s', strongest_postcondition' p P t s' -> Q t s') <->
+      (forall o s s' t, P o s -> exec' o s p (Finished s' t) -> Q t s').
+  Proof.
+    intros; destruct p; simpl; eauto;
+    split; intros;
+    try inversion H1; cleanup;
+    eapply H; eauto;
+    do 2 eexists; eauto.    
+  Qed.
+
+  Theorem scp_complete':
+    forall T (p: prog' T) P (Q:  _ -> Prop),
+      (forall s', strongest_crash_postcondition' p P s' -> Q s') <->
+      (forall o s s', P o s -> exec' o s p (Crashed s') -> Q s').
+  Proof.
+    intros; destruct p; simpl; eauto;
+    split; intros;
+    try inversion H1; cleanup;
+    try split_ors; eapply H; eauto.
+  Qed.
+
+  Theorem wp_complete':
+    forall T (p: prog' T) H Q,
+      (forall o s, H o s -> weakest_precondition' p Q o s) <->
+      (forall o s, H o s -> (exists s' v, exec' o s p (Finished s' v) /\ Q v s')).
+  Proof.
+    intros; destruct p; simpl; eauto;
+    split; intros;
+    specialize H0 with (1:= X);
+    cleanup; eauto;
+    inversion H0; cleanup; eauto.
+  Qed.
+  
+  Theorem wcp_complete':
+    forall T (p: prog' T) H C,
+      (forall o s, H o s -> weakest_crash_precondition' p C o s) <->
+      (forall o s, H o s -> (exists s', exec' o s p (Crashed s') /\ C s')).
+  Proof.
+    unfold weakest_crash_precondition';
+    intros; destruct p; simpl; eauto;
+    split; intros;
+    specialize H0 with (1:= X);
+    cleanup; eauto;
+    inversion H0; cleanup; eauto.
+  Qed.
+
+  Theorem exec_deterministic_wrt_oracle' :
+    forall o s T (p: prog' T) ret1 ret2,
+      exec' o s p ret1 ->
+      exec' o s p ret2 ->
+      ret1 = ret2.
+  Proof.
+    intros; destruct p; simpl in *; cleanup;
+    repeat
+      match goal with
+      | [H: exec' _ _ _ _ |- _] =>
+        inversion H; clear H; cleanup
+      end; eauto.
+  Qed.
+  
+  Definition LoggedDiskOperation :=
+    Build_Operation
+      (list_eq_dec token_dec')
+      prog'
+      exec'
+      weakest_precondition'
+      weakest_crash_precondition'
+      strongest_postcondition'
+      strongest_crash_postcondition'
+      wp_complete'
+      wcp_complete'
+      sp_complete'
+      scp_complete'
+      exec_deterministic_wrt_oracle'.
+
+  Definition LoggedDiskLang := Build_Language LoggedDiskOperation.
+  Definition LoggedDiskHL := Build_HoareLogic LoggedDiskLang.
+
+Notation "| p |" := (Op LoggedDiskOperation p)(at level 60).
+Notation "x <-| p1 ; p2" := (Bind (Op LoggedDiskOperation p1) (fun x => p2))(right associativity, at level 60). 
+Notation "p >> s" := (p s) (right associativity, at level 60, only parsing).
